- [[Induction.pdf]]
- [[Reminder on Factorising]]

Climbing an Infinite Ladder, Can we reach ANY step in this infinite ladder?

Suppose we have an infinite ladder, and we can show: 
1. We can reach the first step of the ladder.
2. If we can reach a particular step of the ladder, then we can reach the next step.

***or, equivalently, any arbitrary rung of the ladder***

# Principle of Mathematical Induction

To prove that ğ‘ƒ(ğ‘›) is true for all positive integers ğ‘›, we complete these steps: 
- Basis Step: Show that ğ‘ƒ(1) is true. 
- Inductive Step:
	- First assume: ğ‘ƒ(ğ‘˜) is true for an arbitrary ğ‘˜ (inductive hypothesis) 
	- Then show: If ğ‘ƒ(ğ‘˜) is true, then ğ‘ƒ(ğ‘˜ + 1) is true for all positive integers ğ‘˜. 
		- That is, show: ğ‘ƒ(ğ‘˜) â†’ ğ‘ƒ(ğ‘˜ + 1) âˆ€ ğ‘˜. 
		- (Using the if-then, or implication symbol "â†’", and for all operator "âˆ€")

***Where "P" is a what is called a proposition.*** 

***A proposition is a statement that must have a truth value; that is, it must be either true or false.*** 

***P(n) is that proposition with a variable that has been set to the value "n".***

***Where k it's really a random number relative to the sequence.***

## Example

### Proof by Induction for $\sum_{i=1}^n I = \frac{n(n+1)}{2}$

**Basis Step**:  
Verify the formula for $(n = 1)$:  
$$
\sum_{i=1}^1 i = 1, \quad \text{and the formula gives: } \frac{1(1+1)}{2} = 1.
$$
Since both sides are equal, the basis step holds.

**Inductive Hypothesis**:  
Assume the formula holds for \( n = k \):  
$$
\sum_{i=1}^k i = \frac{k(k+1)}{2}.
$$

**Inductive Step**:  
Prove the formula for \( n = k+1 \):  
$$
\sum_{i=1}^{k+1} i = \left( \sum_{i=1}^k i \right) + (k+1).
$$
Using the inductive hypothesis:  
$$
\sum_{i=1}^{k+1} i = \frac{k(k+1)}{2} + (k+1).
$$ 
Simplify by factoring \( (k+1) \):  
$$
\sum_{i=1}^{k+1} i = \frac{(k+1)(k+2)}{2}.
$$
This matches the formula for \( n = k+1 \).

**Conclusion**:  
By induction, the formula is true for all positive integers \( n \).


## How to Write the Proof: Template
state clearly what you want to prove, i.e. **P(n)**

basis step
- show that P(1) is true [or, in general, P(b)]

Inductive step: 
- state clearly P(k), i.e. what you are assuming ( the inductive hypothesis) and possible values of k 
- state clearly P(k+1), i.e. what you want to prove
- then show P(k+1) is true using the inductive hypothesis, i.e. P(k) 
- in many cases this involves show that the $lhs = rhs$ of some equation 
- in such cases start manipulating the $lhs$ keeping an eye on rhs $as$ this is where you want to end up look out for where you can use the inductive hypothesis so you can use it

# 3.1. Problem Set: Induction
- [ ] ğŸ”½ 3.1. Problem set: Induction

**Link**
- <https://moodle.gla.ac.uk/mod/book/view.php?id=4586544&chapterid=162862>

1)Â Prove by induction the Theorem that the sum of the first n positive integers is 

$$\frac{n*(n+1)}2$$

*(This was covered in the recorded lecture. Try to do this again from scratch without referring to the lecture/slides)*

**BASIS STEP**
$$n_1=\frac{1+1}2=1$$

**INDUCTIVE HYPOTHESIS**

$$1 + 2 + 3 + â€¦ + k = \frac{n*(n+1)}2$$

**We want to prove:**

$$1 + 2 + 3 + â€¦ + k + k+1=\frac{(k+1)(k+2)}2$$
**RHS**=$\frac{k*(k+1)}2$
**LHS**=$\frac{k(k+1)}2 + k + 1$
**LHS**=$\frac{k^2+2k+2}2$
**LHS**=$\frac{(k+1)(k+2)}2$




2)Â Â Using mathematical induction, prove that the sum of the first n odd numbers is equal to $n^2$. That is, show that:Â $1+3+5+â‹¯+(2n-1)=n^2$

**BASIS STEP**
$$1 = 1^2$$

**INDUCTIVE HYPOTHESIS**

$$1 + 3 + 5 + â€¦ + (2n-1) = n^2$$
**We want to prove:**

$$1 + 3 + 5 + â€¦ + (2n-1) + (2(k+1) - 1) = (k+1)^2$$

**RHS**=$(k+1)^2$
**LHS**=$k^2 + 2k + 1$
**LHS**=$(k+1)^2$

3)Â Prove by induction the Theorem that: Â For any for any nâˆˆâ„¤+ we have n3-n is divisible by 3.  
  
4)Â Using mathematical induction, prove that the sum of first n even positive integers is n(n+1). That is, show that:Â  2+4+6+â‹¯+2n = n(n+1)
# Template
Using mathematical induction, prove that the sum of first n even positive integers is $n(n+1)$. That is, show that:Â  $2+4+6+â‹¯+2n = n(n+1)$.

**BASIS STEP**
$$n_{1}=1(1+1) = n_1=1$$

**INDUCTIVE HYPOTHESIS: 

$$2 + 4 + 6 + â€¦ + 2k = n(n+1)$$

**We want to prove:**

$$2 + 4 + 6 + â€¦ + 2k + 2(k+1)=(k+1)(k+2)$$

**RHS** $=(k+1)(k+2) = k^2+ 3k + 2$ 
**LHS** = $2 + 4 + 6 + â€¦ + 2k + 2(k+1)$

**INDUCTIVE STEP**

**LHS** = $n(n+1)+2(n+1)$
**LHS** = $k^2 + k + 2k + 2$
**LHS** = $k^2 + 3k + 2$

