#pa 

Using mathematical induction, prove that the sum of first n odd numbers is equal to n2 . That is, show that: 

$$1 + 3 + 5 + ‚Ä¶ + (2ùëõ ‚àí 1) = n^2$$
# Base Case (n=1)
**Sub in first value in sequence to prove the formula proves true for the provided sequence.**

For $n=1$:

$$(2*1-1)=1^2$$
$$2-1=1$$
$$1=1$$
Since LHS = RHS the base case holds true.

# Inductive Hypothesis
Assume this holds true for k:

$$1 + 3 + 5 + ‚Ä¶ + (2k ‚àí 1) = k^2$$

# Inductive Step
Prove this holds true for (k+1)

$$1+3+5+‚Ä¶+(2k-1)+(2(k+1)-1)=(k+1)^2$$
$$k^2+(2k+1)=(k+1)^2$$
$$(k+1)^2=(k+1)^2$$
Since RHS = LHS this proves true.